completed Step's definition
--HG--
branch : opt

platform/cito/Optimizer.v
@@ -3,10 +3,15 @@ Require Import Semantics.
 Import SemanticsExpr.
 Import Safety.
 Require Import GeneralTactics.
+Import WDict.
+Import WMake.
+
+Set Implicit Arguments.
 
 Inductive Outcome := 
   | Done : st -> Outcome
-  | ToCall : W -> W -> Statement -> st -> Outcome.
+  | ToCall : W -> W -> Statement -> st -> Outcome
+  | ToMalloc : string -> W -> Statement -> st -> Outcome.
                    
 Inductive Step : Statement -> st -> Outcome -> Prop :=
   | Skip : forall v, Step Syntax.Skip v (Done v)
@@ -21,7 +26,64 @@ Inductive Step : Statement -> st -> Outcome -> Prop :=
       let v := (vs, arrs) in
       let f_v := exprDenote f vs in
       let arg_v := exprDenote arg vs in
-      Step (Syntax.Call f arg) v (ToCall f_v arg_v Syntax.Skip v).
+      Step (Syntax.Call f arg) v (ToCall f_v arg_v Syntax.Skip v)
+  | Malloc : forall var size vs arrs,
+      let v := (vs, arrs) in
+      let size_v := exprDenote size vs in
+      Step (Syntax.Malloc var size) v (ToMalloc var size_v Syntax.Skip v)
+  | IfTrue : forall v v' cond t f, 
+      wneb (exprDenote cond (fst v)) $0 = true -> 
+      Step t v v' -> 
+      Step (Conditional cond t f) v v'
+  | IfFalse : forall v v' cond t f, 
+      wneb (exprDenote cond (fst v)) $0 = false -> 
+      Step f v v' -> 
+      Step (Conditional cond t f) v v'
+  | WhileFalse : forall v cond body, 
+      wneb (exprDenote cond (fst v)) $0 = false -> 
+      Step (Loop cond body) v (Done v)
+  | WhileTrue1 : forall v v' v'' cond body, 
+      let loop := Loop cond body in
+      wneb (exprDenote cond (fst v)) $0 = true -> 
+      Step body v (Done v') -> 
+      Step loop v' v'' -> 
+      Step loop v v''
+  | WhileTrue2 : forall cond body v f x s' v', 
+      let loop := Loop cond body in
+      wneb (exprDenote cond (fst v)) $0 = true -> 
+      Step body v (ToCall f x s' v') -> 
+      Step loop v (ToCall f x (Syntax.Seq s' loop) v')
+  | Assign : forall var value vs arrs, 
+      let v := (vs, arrs) in
+      let value_v := exprDenote value vs in
+      Step (Syntax.Assignment var value) v (Done (Locals.upd vs var value_v, arrs))
+  | Read : forall var arr idx vs (arrs : arrays),
+      let v := (vs, arrs) in
+      let arr_v := exprDenote arr vs in
+      let idx_v := exprDenote idx vs in
+      safe_access arrs arr_v idx_v -> 
+      let value_v := Array.sel (snd arrs arr_v) idx_v in  
+      Step (Syntax.ReadAt var arr idx) v (Done (Locals.upd vs var value_v, arrs))
+  | Write : forall arr idx value vs (arrs : arrays), 
+      let v := (vs, arrs) in
+      let arr_v := exprDenote arr vs in
+      let idx_v := exprDenote idx vs in
+      safe_access arrs arr_v idx_v ->
+      let value_v := exprDenote value vs in
+      let new_arr := Array.upd (snd arrs arr_v) idx_v value_v in
+      Step (Syntax.WriteAt arr idx value) v (Done (vs, (fst arrs, upd (snd arrs) arr_v new_arr)))  | Len : forall var arr vs arrs,
+      let v := (vs, arrs) in
+      let arr_v := exprDenote arr vs in
+      arr_v %in fst arrs ->
+      let len := natToW (length (snd arrs arr_v)) in
+      Step (Syntax.Len var arr) v (Done (Locals.upd vs var len, arrs))
+  | Free : forall arr vs (arrs : arrays),
+      let v := (vs, arrs) in
+      let arr_v := exprDenote arr vs in
+      arr_v %in fst arrs ->
+      Step (Syntax.Free arr) v (Done (vs, (fst arrs %- arr_v, snd arrs)))
+.
+
 
 Lemma Step_deterministic : forall s v v1 v2, Step s v v1 -> Step s v v2 -> v1 = v2.
   admit.
@@ -36,6 +98,10 @@ CoInductive bisimilar s t : Prop :=
          (exists f x s' t' v',
             Step s v (ToCall f x s' v') /\ 
             Step t v (ToCall f x t' v') /\ 
+            bisimilar s' t') \/
+         (exists r x s' t' v',
+            Step s v (ToMalloc r x s' v') /\
+            Step t v (ToMalloc r x s' v') /\
             bisimilar s' t')) ->
       bisimilar s t.
 
@@ -53,14 +119,21 @@ Section bisimilar_coind.
         (exists f x s' t' v', 
            Step s v (ToCall f x s' v') /\ 
            Step t v (ToCall f x t' v') /\ 
+           R s' t') \/
+        (exists r x s' t' v',
+           Step s v (ToMalloc r x s' v') /\
+           Step t v (ToMalloc r x s' v') /\
            R s' t').
 
   Hint Constructors bisimilar.
 
   Theorem bisimilar_coind : forall s t, R s t -> bisimilar s t.
-    cofix; intros; econstructor; intros; specialize (is_bisimulation _ _ H v); destruct is_bisimulation; clear is_bisimulation.
+    cofix; intros; econstructor; intros; specialize (is_bisimulation H v).
+    destruct is_bisimulation; clear is_bisimulation.
     left; eauto.
-    right; openhyp; do 5 eexists; eauto.
+    openhyp.
+    right; left; openhyp; do 5 eexists; eauto.
+    right; right; openhyp; do 5 eexists; eauto.
   Qed.
 
 End bisimilar_coind.
@@ -82,23 +155,35 @@ Section Functions.
   Variable fs : W -> option Callee.
 
   Inductive StepsTo : Statement -> st -> st -> Prop :=
-    | NoCall :
-        forall s v v',
-          Step s v (Done v') ->
-          StepsTo s v v'
-    | HasForeign :
+  | NoCall :
+      forall s v v',
+        Step s v (Done v') ->
+        StepsTo s v v'
+  | HasForeign :
       forall s v f x s' v' spec v'' v''',
         Step s v (ToCall f x s' v') ->
         fs f = Some (Foreign spec) -> 
         spec {| Arg := x; InitialHeap := snd v'; FinalHeap := snd v'' |} ->
         StepsTo s' v'' v''' ->
         StepsTo s v v'''
-    | HasInternal :
+  | HasInternal :
       forall s v f x s' v' body vs_arg v'' v''',
         Step s v (ToCall f x s' v') ->
         fs f = Some (Internal body) -> 
         Locals.sel vs_arg "__arg" = x ->
         StepsTo body (vs_arg, snd v') v'' ->
+        StepsTo s' v'' v''' ->
+        StepsTo s v v'''
+  | HasMalloc : 
+      forall s v var x s' v' addr ls v''',
+        Step s v (ToMalloc var x s' v') ->
+        let vs := fst v' in
+        let arrs := snd v' in
+        ~ (addr %in fst arrs) ->
+        let size_v := wordToNat x in
+        goodSize (size_v + 2) ->
+        length ls = size_v ->
+        let v'' := (Locals.upd vs var addr, (fst arrs %+ addr, upd (snd arrs) addr ls)) in
         StepsTo s' v'' v''' ->
         StepsTo s v v'''.
 
@@ -116,6 +201,7 @@ Lemma correct_StepsTo : forall sfs s v v', StepsTo sfs s v v' -> forall tfs t, b
   inversion H0; subst; specialize (H2 v); openhyp.
   econstructor; eapply Step_deterministic in H2; [ | eapply H]; injection H2; intros; subst; eauto.
   eapply Step_deterministic in H2; [ | eapply H]; discriminate.
+  eapply Step_deterministic in H2; [ | eapply H]; discriminate.
 
   inversion H3; subst; specialize (H5 v); openhyp.
   eapply Step_deterministic in H5; [ | eapply H]; discriminate.
@@ -126,6 +212,8 @@ Lemma correct_StepsTo : forall sfs s v v', StepsTo sfs s v v' -> forall tfs t, b
   econstructor 2; eauto.
   eapply H12; eauto.
 
+  eapply Step_deterministic in H5; [ | eapply H]; discriminate.
+
   inversion H4; subst; specialize (H6 v); openhyp.
   eapply Step_deterministic in H1; [ | eapply H]; discriminate.
   generalize H5; intro; specialize (H5 f); openhyp.
@@ -133,6 +221,19 @@ Lemma correct_StepsTo : forall sfs s v v', StepsTo sfs s v v' -> forall tfs t, b
   rewrite H0 in *; injection H5; intros; subst; inversion H10; subst.
   eapply Step_deterministic in H1; [ | eapply H]; injection H1; intros; subst.
   econstructor 3; eauto.
+
+  eapply Step_deterministic in H1; [ | eapply H]; discriminate.
+
+  inversion H4; subst; specialize (H6 v); openhyp.
+  eapply Step_deterministic in H6; [ | eapply H]; discriminate.
+  eapply Step_deterministic in H6; [ | eapply H]; discriminate.
+(*here*)
+  generalize H5; intro; specialize (H5 f); openhyp.
+  rewrite H0 in *; discriminate.
+  rewrite H0 in *; injection H5; intros; subst; inversion H10; subst.
+  eapply Step_deterministic in H1; [ | eapply H]; injection H1; intros; subst.
+  econstructor 3; eauto.
+
 Qed.
 Hint Resolve correct_StepsTo.
 
